Implement Stackless JMPZ

Uppaal_Networks/AbsInt/State_Stackless.thy
@@ -89,9 +89,29 @@ fun \<gamma>_stackless :: "'a stackless \<Rightarrow> collect_state set" where
   "\<gamma>_stackless None = \<bottom>" |
   "\<gamma>_stackless (Some (Stackless aregs aflag)) = {(stack, rstate, flag, nl). rstate \<in> \<gamma>_regs aregs \<and> flag \<in> \<gamma>_power_bool aflag}"
 
+fun step_stackless_base :: "instr \<Rightarrow> addr \<Rightarrow> 'a stackless_base \<Rightarrow> 'a stackless state_map" where
+  "step_stackless_base (JMPZ target) pc (Stackless regs BTrue) = single (Suc pc) (Some (Stackless regs BTrue))" |
+  "step_stackless_base (JMPZ target) pc (Stackless regs BFalse) = single target (Some (Stackless regs BFalse))" |
+  "step_stackless_base (JMPZ target) pc (Stackless regs BBoth) = deep_merge {(target, Some (Stackless regs BBoth)), (Suc pc, Some (Stackless regs BBoth))}" |
+  "step_stackless_base _ _ _ = \<top>"
+
 fun step_stackless :: "('a::absword) stackless astep" where
   "step_stackless _ _ None = \<bottom>" |
-  "step_stackless _ _ _    = \<top>"
+  "step_stackless op pc (Some a) = step_stackless_base op pc a"
+
+lemma gamma_stackless_mono:
+  assumes "a \<le> b"
+  shows "\<gamma>_stackless a \<subseteq> \<gamma>_stackless b"
+proof (intro Set.subsetI)
+  fix x assume ass: "x \<in> \<gamma>_stackless a"
+  from ass obtain aregs aflag where asplit: "a = Some (Stackless aregs aflag)" by (metis \<gamma>_stackless.elims empty_iff)
+  from this assms obtain bregs bflag where bsplit: "b = Some (Stackless bregs bflag)" by (metis \<gamma>_stackless.cases less_eq_option.simps(2))
+  from ass obtain stack rstate flag nl where xsplit: "x = (stack, rstate, flag, nl)" using prod_cases4 by blast 
+  from assms asplit bsplit have fine_le: "aregs \<le> bregs" "aflag \<le> bflag" by auto
+  from asplit xsplit ass have "rstate \<in> \<gamma>_regs aregs \<and> flag \<in> \<gamma>_power_bool aflag" by simp
+  from this fine_le have "rstate \<in> \<gamma>_regs bregs" "flag \<in> \<gamma>_power_bool bflag" using mono_gamma_power_bool mono_gamma_regs by (blast, blast)
+  from this bsplit xsplit show "x \<in> \<gamma>_stackless b" by simp
+qed
 
 lemma gamma_stackless_top: "\<gamma>_stackless \<top> = \<top>"
 proof -
@@ -100,62 +120,114 @@ proof -
 qed
 
 lemma step_stackless_nonbot_correct:
-  assumes "a \<noteq> \<bottom>"
-  shows "lookup (collect_step op ipc (\<gamma>_stackless a)) pc \<le> \<gamma>_stackless (lookup (step_stackless op ipc a) pc)"
-proof (cases op)
-  case (JMPZ x1)
-  then show ?thesis using assms by auto
-next
-  case ADD
-  then show ?thesis using assms by auto
-next
-  case NOT
-  then show ?thesis using assms by auto
-next
-  case AND
-  then show ?thesis using assms by auto
-next
-  case LT
-  then show ?thesis using assms by auto
-next
-  case LE
-  then show ?thesis using assms by auto
-next
-  case EQ
-  then show ?thesis using assms by auto
-next
-  case (PUSH x8)
-  then show ?thesis using assms by auto
-next
-  case POP
-  then show ?thesis using assms by auto
-next
-  case (LID x10)
-  then show ?thesis using assms by auto
-next
-  case STORE
-  then show ?thesis using assms by auto
-next
-  case (STOREI x121 x122)
-  then show ?thesis using assms by auto
-next
-  case COPY
-  then show ?thesis using assms by auto
-next
-  case CALL
-  then show ?thesis using assms by auto
-next
-  case RETURN
-  then show ?thesis using assms by auto
-next
-  case HALT
-  then show ?thesis using assms by auto
-next
-  case (STOREC x171 x172)
-  then show ?thesis using assms by auto
-next
-  case (SETF x18)
-  then show ?thesis using assms by auto
+  assumes "ost \<in> lookup (collect_step op ipc (\<gamma>_stackless (Some (Stackless iaregs iaflag)))) opc"
+  shows "ost \<in> \<gamma>_stackless (lookup (step_stackless op ipc (Some (Stackless iaregs iaflag))) opc)"
+proof -
+  obtain ocstack ocregs ocflag ocrs where ost_split: "ost = (ocstack, ocregs, ocflag, ocrs)" by (rule prod_cases4)
+
+  let ?ists = "\<gamma>_stackless (Some (Stackless iaregs iaflag))"
+  from assms have "\<exists>ist\<in>?ists. step op (ipc, ist) = Some (opc, ost)" by simp
+  from this obtain ist where ist_step: "ist \<in> ?ists" "step op (ipc, ist) = Some (opc, ost)" ..
+  obtain icstack icregs icflag icrs where ist_split: "ist = (icstack, icregs, icflag, icrs)" by (rule prod_cases4)
+
+  from ist_split ist_step ost_split have ist_split_step:
+    "(icstack, icregs, icflag, icrs) \<in> ?ists"
+    "step op (ipc, (icstack, icregs, icflag, icrs)) = Some (opc, (ocstack, ocregs, ocflag, ocrs))" by auto
+
+  (* more properties can be added here if \<gamma>_stackless gets updated *)
+  from ist_step(1) ist_split have ist_props: "icregs \<in> \<gamma>_regs iaregs" "icflag \<in> \<gamma>_power_bool iaflag" by auto
+
+  show ?thesis 
+  proof (cases op)
+    case (JMPZ target)
+    from JMPZ ist_split_step have stack_preserve: "ocstack = icstack" using step_jmpz(1) by blast
+    from JMPZ ist_split_step have regs_preserve: "ocregs = icregs" using step_jmpz(2) by blast
+    from JMPZ ist_split_step have flag_preserve: "ocflag = icflag" using step_jmpz(3) by blast
+    from JMPZ ist_split_step have rs_preserve: "ocrs = icrs" using step_jmpz(4) by blast
+    show ?thesis
+    proof (cases iaflag)
+      case BTrue
+      from this have "icflag = True" using ist_props by simp
+      from this JMPZ ist_split_step(2) have "opc = Suc ipc" using step_jmpz_true(4) by blast
+      from this BTrue JMPZ have "lookup (step_stackless op ipc (Some (Stackless iaregs iaflag))) opc = Some (Stackless iaregs iaflag)" using single_lookup by simp
+      then show ?thesis using ist_split flag_preserve ist_step(1) ost_split regs_preserve by simp
+    next
+      case BFalse
+      from this have "icflag = False" using ist_props by simp
+      from this JMPZ ist_split_step(2) have "opc = target" using step_jmpz_false(4) by blast
+      from this BFalse JMPZ have "lookup (step_stackless op ipc (Some (Stackless iaregs iaflag))) opc = Some (Stackless iaregs iaflag)" using single_lookup by simp
+      then show ?thesis using ist_split flag_preserve ist_step(1) ost_split regs_preserve by simp
+    next
+      case BBoth
+      then show ?thesis
+      proof (cases icflag)
+        case True
+        from this JMPZ ist_split_step(2) have "opc = Suc ipc" using step_jmpz_true(4) by (metis(full_types))
+        from this BBoth JMPZ have lookup: "Some (Stackless iaregs iaflag) \<le> lookup (step_stackless op ipc (Some (Stackless iaregs iaflag))) opc" using deep_merge_lookup
+          by (metis insert_iff step_stackless.simps(2) step_stackless_base.simps(3))
+        have "ost \<in> \<gamma>_stackless (Some (Stackless iaregs iaflag))" using ist_split flag_preserve ist_step(1) ost_split regs_preserve by simp
+        from this lookup show ?thesis using gamma_stackless_mono by blast
+      next
+        case False
+        from this JMPZ ist_split_step(2) have "opc = target" using step_jmpz_false(4) by (metis(full_types))
+        from this BBoth JMPZ have lookup: "Some (Stackless iaregs iaflag) \<le> lookup (step_stackless op ipc (Some (Stackless iaregs iaflag))) opc" using deep_merge_lookup
+          by (metis insert_iff step_stackless.simps(2) step_stackless_base.simps(3))
+        have "ost \<in> \<gamma>_stackless (Some (Stackless iaregs iaflag))" using ist_split flag_preserve ist_step(1) ost_split regs_preserve by simp
+        from this lookup show ?thesis using gamma_stackless_mono by blast
+      qed
+    qed
+  next
+    case ADD
+    then show ?thesis by auto
+  next
+    case NOT
+    then show ?thesis by auto
+  next
+    case AND
+    then show ?thesis by auto
+  next
+    case LT
+    then show ?thesis by auto
+  next
+    case LE
+    then show ?thesis by auto
+  next
+    case EQ
+    then show ?thesis by auto
+  next
+    case (PUSH x8)
+    then show ?thesis by auto
+  next
+    case POP
+    then show ?thesis by auto
+  next
+    case (LID x10)
+    then show ?thesis by auto
+  next
+    case STORE
+    then show ?thesis by auto
+  next
+    case (STOREI x121 x122)
+    then show ?thesis by auto
+  next
+    case COPY
+    then show ?thesis by auto
+  next
+    case CALL
+    then show ?thesis by auto
+  next
+    case RETURN
+    then show ?thesis by auto
+  next
+    case HALT
+    then show ?thesis by auto
+  next
+    case (STOREC x171 x172)
+    then show ?thesis by auto
+  next
+    case (SETF x18)
+    then show ?thesis by auto
+  qed
 qed
 
 end
@@ -165,22 +237,22 @@ sublocale AbsWord \<subseteq> AbsInt
     and ai_step = step_stackless
 proof (standard, goal_cases)
   case (1 a b)
-  then show ?case
-  proof (intro Set.subsetI)
-    fix x assume ass: "x \<in> \<gamma>_stackless a"
-    from ass obtain aregs aflag where asplit: "a = Some (Stackless aregs aflag)" by (metis \<gamma>_stackless.elims empty_iff)
-    from this 1 obtain bregs bflag where bsplit: "b = Some (Stackless bregs bflag)" by (metis \<gamma>_stackless.cases less_eq_option.simps(2))
-    from ass obtain stack rstate flag nl where xsplit: "x = (stack, rstate, flag, nl)" using prod_cases4 by blast 
-    from 1 asplit bsplit have fine_le: "aregs \<le> bregs" "aflag \<le> bflag" by auto
-    from asplit xsplit ass have "rstate \<in> \<gamma>_regs aregs \<and> flag \<in> \<gamma>_power_bool aflag" by simp
-    from this fine_le have "rstate \<in> \<gamma>_regs bregs" "flag \<in> \<gamma>_power_bool bflag" using mono_gamma_power_bool mono_gamma_regs by (blast, blast)
-    from this bsplit xsplit show "x \<in> \<gamma>_stackless b" by simp
-  qed
+  then show ?case by (rule gamma_stackless_mono)
 next
   case 2 show ?case by (rule gamma_stackless_top)
 next
   case (3 op ipc a pc)
-  then show ?case using step_stackless_nonbot_correct by (cases "a = \<bottom>", simp)
+  then show ?case using step_stackless_nonbot_correct
+  proof (cases "a = \<bottom>")
+    case True
+    then show ?thesis by simp
+  next
+    case False
+    have "lookup (collect_step op ipc (\<gamma>_stackless (Some (Stackless regs flag)))) pc
+          \<le> \<gamma>_stackless (lookup (step_stackless op ipc (Some (Stackless regs flag))) pc)" for regs flag
+      using step_stackless_nonbot_correct by blast
+    from this False show ?thesis by (metis \<gamma>_stackless.elims bot_option_def)
+  qed
 next
   case (4 op ipc pc)
   then show ?case by simp
